

Limit of a function

a) $f(x) = \frac{x^2 - x - 2}{6 - 2x}$.

First, we determine the domain

$$D_f = \mathbb{R} \setminus \{3\}.$$

Now we compute the limits at the boundary points of the domain. Start with infinities:

$$\begin{aligned} \lim_{x \rightarrow +\infty} \frac{x^2 - x - 2}{6 - 2x} &= \lim_{x \rightarrow +\infty} \frac{x}{x} \frac{x - 1 - 2/x}{6/x - 2} \\ &\stackrel{\text{Limit arithmetics}}{=} \frac{\lim_{x \rightarrow +\infty} (x - 1 - 2/x)}{\lim_{x \rightarrow +\infty} (6/x - 2)} \\ &= +\infty / (-2) \\ &= -\infty, \end{aligned}$$

$$\begin{aligned} \lim_{x \rightarrow -\infty} \frac{x^2 - x - 2}{6 - 2x} &= \lim_{x \rightarrow -\infty} \frac{x}{x} \frac{x - 1 - 2/x}{6/x - 2} \\ &\stackrel{\text{Limit arithmetics}}{=} \frac{\lim_{x \rightarrow -\infty} (x - 1 - 2/x)}{\lim_{x \rightarrow -\infty} (6/x - 2)} \\ &= -\infty / (-2) \\ &= +\infty. \end{aligned}$$

Next, compute one-sided limits for $x = 3$:

$$\begin{aligned} \lim_{x \rightarrow 3^+} \frac{x^2 - x - 2}{6 - 2x} &= \frac{4}{0^-} = -\infty, \\ \lim_{x \rightarrow 3^-} \frac{x^2 - x - 2}{6 - 2x} &= \frac{4}{0^+} = +\infty. \end{aligned}$$

Intercepts can be found in a standard way. For the y -intercept, let $x = 0$:

$$P_y = [0, -1/3].$$

For the x -intercepts, set $y = 0$, so we solve

$$x^2 - x - 2 = 0,$$

which is a quadratic equation with roots $x_1 = -1$ and $x_2 = 2$. The two intercepts with the x -axis are therefore:

$$P_{x1} = [-1, 0], \quad P_{x2} = [2, 0].$$

Derivatives

a) $f(x) = \sqrt{x^4 + 5x^2}$

We differentiate as a composite function (the outer function is the square root and the inner function is the polynomial $x^4 + 5x^2$). Therefore,

$$f'(x) = \frac{1}{2\sqrt{x^4 + 5x^2}} \cdot (4x^3 + 10x) = \frac{2x^3 + 5x}{\sqrt{x^4 + 5x^2}}.$$

b) $f(x) = e^{3-5x}(x^4 - 3x + 4)$

We differentiate as a product of two functions: an exponential (which is itself composite with the inner function $3 - 5x$) and the polynomial $x^4 - 3x + 4$. Thus,

$$\begin{aligned} f'(x) &= (e^{3-5x})'(x^4 - 3x + 4) + e^{3-5x}(x^4 - 3x + 4)' \\ &= e^{3-5x}(-5)(x^4 - 3x + 4) + e^{3-5x}(4x^3 - 3) \\ &= e^{3-5x}(-5x^4 + 15x - 20 + 4x^3 - 3) \\ &= e^{3-5x}(-5x^4 + 4x^3 + 15x - 23). \end{aligned}$$

c) $f(x) = (3x^2 + 5x)^3$

We differentiate as a composite function (outer function is the cube, inner function is the polynomial $3x^2 + 5x$). Thus,

$$f'(x) = 3(3x^2 + 5x)^2 \cdot (6x + 5).$$

It is correct to leave the result in this simplified factored form. If we expand:

$$(3x^2 + 5x)^2 = 9x^4 + 30x^3 + 25x^2,$$

so

$$\begin{aligned}f'(x) &= (9x^4 + 30x^3 + 25x^2)(6x + 5) \\&= 54x^5 + 45x^4 + 180x^4 + 150x^3 + 150x^3 + 125x^2 \\&= 54x^5 + 225x^4 + 300x^3 + 125x^2.\end{aligned}$$

d) $f(x) = \frac{\ln x}{2x^2 + 5x}$

This is a quotient of two functions $f_1(x) = \ln x$ and $f_2(x) = 2x^2 + 5x$, so by the quotient rule:

$$f'(x) = \frac{\frac{1}{x}(2x^2 + 5x) - (4x + 5) \ln x}{(2x^2 + 5x)^2}.$$

We simplify:

$$\frac{1}{x}(2x^2 + 5x) = 2x + 5,$$

and

$$(2x^2 + 5x)^2 = 4x^4 + 20x^3 + 25x^2.$$

Final result:

$$f'(x) = \frac{2x + 5 - (4x + 5) \ln x}{4x^4 + 20x^3 + 25x^2}.$$